Cslib.lean
@@ -85,6 +85,7 @@ public import Cslib.Foundations.Logic.Axioms
 public import Cslib.Foundations.Logic.Connectives
 public import Cslib.Foundations.Logic.InferenceSystem
 public import Cslib.Foundations.Logic.LogicalEquivalence
+public import Cslib.Foundations.Logic.Metalogic.Chronicle.SinceSeedConsistency
 public import Cslib.Foundations.Logic.Metalogic.Consistency
 public import Cslib.Foundations.Logic.Metalogic.DeductionCharacterization
 public import Cslib.Foundations.Logic.Metalogic.DeductionHelpers
